theories/Core/Completeness/TermStructureCases.v
@@ -1,0 +1,97 @@
+From Coq Require Import RelationClasses.
+From Mcltt Require Import Base LibTactics LogicalRelation System.
+Import Domain_Notations.
+
+Lemma rel_exp_sub_cong : forall {Δ M M' A σ σ' Γ},
+    {{ Δ ⊨ M ≈ M' : A }} ->
+    {{ Γ ⊨s σ ≈ σ' : Δ }} ->
+    {{ Γ ⊨ M[σ] ≈ M'[σ'] : A[σ] }}.
+Proof.
+  intros * [env_relΔ] [env_relΓ].
+  destruct_conjs.
+  per_ctx_env_irrel_rewrite.
+  eexists.
+  eexists; try eassumption.
+  eexists.
+  intros.
+  assert (env_relΓ p' p) by (eapply per_env_sym; eauto).
+  assert (env_relΓ p p) by (eapply per_env_trans; eauto).
+  (on_all_hyp: fun H => destruct_rel_by_assumption env_relΓ H).
+  per_univ_elem_irrel_rewrite.
+  assert (env_relΔ o o0) by (eapply per_env_trans; [eauto | | eapply per_env_sym]; revgoals; eauto).
+  (on_all_hyp: fun H => destruct_rel_by_assumption env_relΔ H).
+  destruct_by_head rel_exp.
+  destruct_by_head rel_typ.
+  per_univ_elem_irrel_rewrite.
+  eexists.
+  split; [> econstructor; only 1-2: econstructor; eauto ..].
+Qed.
+
+Lemma rel_exp_conv : forall {Γ M M' A A' i},
+    {{ Γ ⊨ M ≈ M' : A }} ->
+    {{ Γ ⊨ A ≈ A' : Type@i }} ->
+    {{ Γ ⊨ M ≈ M' : A' }}.
+Proof.
+  intros * [env_relΓ] [env_relΓ'].
+  destruct_conjs.
+  per_ctx_env_irrel_rewrite.
+  eexists.
+  eexists; try eassumption.
+  eexists.
+  intros.
+  assert (env_relΓ p p) by (eapply per_env_trans; eauto; eapply per_env_sym; eauto).
+  (on_all_hyp: fun H => destruct_rel_by_assumption env_relΓ H).
+  destruct_by_head rel_exp.
+  destruct_by_head rel_typ.
+  inversion_by_head (eval_exp {{{ Type@i }}}); subst.
+  per_univ_elem_irrel_rewrite.
+  match_by_head1 per_univ_elem ltac:(fun H => invert_per_univ_elem H; let n := numgoals in guard n <= 1); clear_refl_eqs.
+  destruct_conjs.
+  per_univ_elem_irrel_rewrite.
+  eexists.
+  split; [> econstructor; eauto ..].
+  eapply per_univ_trans; [eapply per_univ_sym |]; eauto.
+Qed.
+
+Lemma rel_exp_sym : forall {Γ M M' A},
+    {{ Γ ⊨ M ≈ M' : A }} ->
+    {{ Γ ⊨ M' ≈ M : A }}.
+Proof.
+  intros * [env_relΓ].
+  destruct_conjs.
+  econstructor.
+  eexists; try eassumption.
+  eexists.
+  intros ? ? equiv_p_p'.
+  assert (env_relΓ p' p) by (eapply per_env_sym; eauto).
+  (on_all_hyp: fun H => destruct_rel_by_assumption env_relΓ H); destruct_conjs.
+  destruct_by_head rel_exp.
+  destruct_by_head rel_typ.
+  per_univ_elem_irrel_rewrite.
+  eexists.
+  split; econstructor; eauto.
+  eapply per_elem_sym; eauto.
+Qed.
+
+Lemma rel_exp_trans : forall {Γ M1 M2 M3 A},
+    {{ Γ ⊨ M1 ≈ M2 : A }} ->
+    {{ Γ ⊨ M2 ≈ M3 : A }} ->
+    {{ Γ ⊨ M1 ≈ M3 : A }}.
+Proof.
+  intros * [env_relΓ] [env_relΓ'].
+  destruct_conjs.
+  per_ctx_env_irrel_rewrite.
+  econstructor.
+  eexists; try eassumption.
+  eexists.
+  intros ? ? equiv_p_p'.
+  assert (env_relΓ p' p) by (eapply per_env_sym; eauto).
+  assert (env_relΓ p' p') by (eapply per_env_trans; eauto).
+  (on_all_hyp: fun H => destruct_rel_by_assumption env_relΓ H); destruct_conjs.
+  destruct_by_head rel_exp.
+  destruct_by_head rel_typ.
+  per_univ_elem_irrel_rewrite.
+  eexists.
+  split; econstructor; eauto.
+  eapply per_elem_trans; eauto.
+Qed.
