theories/Core/Completeness/VariableCases.v
@@ -1,0 +1,43 @@
+From Coq Require Import Relations.
+From Mcltt Require Import Base LibTactics LogicalRelation System.
+Import Domain_Notations.
+
+Lemma valid_lookup : forall {Γ x A env_rel}
+                        (equiv_Γ_Γ : {{ EF Γ ≈ Γ ∈ per_ctx_env ↘ env_rel }}),
+    {{ # x : A ∈ Γ }} ->
+    exists i,
+    forall p p' (equiv_p_p' : {{ Dom p ≈ p' ∈ env_rel }}),
+    exists elem_rel,
+      rel_typ i A p A p' elem_rel /\ rel_exp elem_rel {{{ # x }}} p {{{ # x }}} p'.
+Proof with solve [repeat econstructor; mauto].
+  intros.
+  assert {{ # x : A ∈ Γ }} as HxinΓ by mauto.
+  remember Γ as Δ eqn:HΔΓ in HxinΓ, equiv_Γ_Γ at 2. clear HΔΓ. rename equiv_Γ_Γ into equiv_Γ_Δ.
+  remember A as A' eqn:HAA' in HxinΓ |- * at 2. clear HAA'.
+  gen Δ A' env_rel.
+  induction H; intros * equiv_Γ_Δ H0; inversion H0; subst; clear H0; inversion_clear equiv_Γ_Δ; subst; simpl in *.
+  - eexists.
+    intros ? ? [equiv_p_drop_p'_drop].
+    exists (head_rel _ _ equiv_p_drop_p'_drop).
+    (on_all_hyp: fun H => destruct_rel_by_assumption tail_rel H); destruct_conjs.
+    split; econstructor...
+  - specialize (IHctx_lookup _ _ _ equiv_Γ_Γ' H2) as [j ?]; destruct_conjs.
+    eexists.
+    intros ? ? [equiv_p_drop_p'_drop].
+    (on_all_hyp: fun H => destruct_rel_by_assumption tail_rel H); destruct_conjs.
+    eexists.
+    destruct_by_head rel_mod_eval.
+    destruct_by_head rel_exp.
+    inversion_by_head (eval_exp {{{ # n }}}); subst.
+    split; econstructor; simpl...
+Qed.
+
+Lemma valid_var : forall {Γ x A},
+    {{ ⊨ Γ }} ->
+    {{ # x : A ∈ Γ }} ->
+    {{ Γ ⊨ # x : A }}.
+Proof.
+  intros * [? equiv_Γ_Γ] ?.
+  econstructor.
+  unshelve epose proof (valid_lookup equiv_Γ_Γ _); mauto.
+Qed.
